deps/poulet4/lib/P4cub/BigStepTypeSoundness.v
@@ -4,7 +4,8 @@ Require Import Poulet4.P4cub.BigStep.
 
 Module P := Poulet4.P4cub.AST.P4cub.
 Module E := P.Expr.
-Module S := P.Stmt.
+Module ST := P.Stmt.
+Module PS := P.Parser.ParserState.
 Module V := Val.
 Import P.P4cubNotations.
 
@@ -182,4 +183,34 @@ Section BigStepTheorems.
           end; eauto 3.
     Qed.
   End LVProgress.
+
+  Section ParserExprProgress.
+    Hint Constructors parser_expr_big_step : core.
+
+    Theorem parser_expr_progress : forall sts errs Γ ϵ (e : PS.e tags_t),
+      envs_sound Γ ϵ errs -> ⟅ sts, errs, Γ ⟆ ⊢ e -> exists st, ⦑ ϵ, e ⦒ ⇓ st.
+    Proof.
+      intros sts errs Γ ϵ e Hsound He.
+      induction He using custom_check_prsrexpr_ind; eauto.
+      assert (Hvcases :
+                exists vcases, Forall2
+                            (fun epe vps =>
+                               let e := fst epe in
+                               let v := fst vps in
+                               let pe := snd epe in
+                               let ps := snd vps in
+                               ⦑ ϵ, pe ⦒ ⇓ ps /\ ⟨ ϵ, e ⟩ ⇓ v)
+                            cases vcases).
+      { clear e def H He IHHe.
+        ind_list_Forall; repeat inv_Forall_cons;
+        try invert_cons_predfs; eauto 2; intuition.
+        eapply expr_big_step_progress in H0 as [v ?];
+        destruct H1 as [st ?]; destruct H3 as [vcases ?]; eauto 1.
+        exists ((v,st) :: vcases); auto 3. }
+      eapply expr_big_step_progress in H as [v ?]; eauto 1.
+      pose proof IHHe Hsound as [dst ?].
+      destruct Hvcases as [vcases ?].
+      exists (match F.get v vcases with None => dst | Some st => st end); auto 2.
+    Qed.
+  End ParserExprProgress.
 End BigStepTheorems.
